NLustre/NLSyntax.v
@@ -104,6 +104,8 @@ Module Type NLSYNTAX
                          ~ In out (vars_defined (filter is_fby n_eqs));
         n_nodup : NoDupMembers (n_in ++ n_vars ++ n_out);
         n_good  : Forall ValidId (n_in ++ n_vars ++ n_out)
+                  /\ Forall valid (vars_defined (filter is_app n_eqs))
+                  /\ valid n_name
       }.
 
   (** ** Program *)
