NLustreToObc/Translation.v
@@ -53,7 +53,7 @@ Module Type TRANSLATION
     | EqDef _ _ _   => acc
     | EqApp xs _ f _ =>
       match xs with
-      | [] => (fst acc, snd acc)
+      | [] => acc
       | x :: _ =>
         (fst acc, (x, f) :: snd acc)
       end
@@ -757,12 +757,9 @@ Module Type TRANSLATION
                          m_in   := idty n.(n_in);
                          m_vars := idty dvars;
                          m_out  := idty n.(n_out);
-                         m_body := translate_eqns mems n.(n_eqs);
-                         m_nodupvars := _;
-                         m_good      := _
+                         m_body := translate_eqns mems n.(n_eqs)
                       |};
-                      reset_method n.(n_eqs) ];
-       c_nodup   := _
+                      reset_method n.(n_eqs) ]
     |}.
   (* =end= *)
   Next Obligation.
@@ -814,6 +811,12 @@ Module Type TRANSLATION
     constructor; auto using NoDup.
     inversion_clear 1; auto.
     now apply reset_not_step.
+  Qed.
+  Next Obligation.
+    pose proof n.(n_good) as (? & ValidApp & ?).
+    split; auto.
+    rewrite <-fst_gather_eqs_var_defined, Forall_app, Forall_map in ValidApp.
+    tauto.
   Qed.
 
   (* =translate= *)
